Save progress

theories/normalization.v
@@ -1,10 +1,32 @@
 Require Import Autosubst2.syntax ssreflect ssrbool.
-From Hammer Require Import Tactics.
+From Hammer Require Import Tactics Hammer.
 From stdpp Require Import relations (rtc(..), rtc_transitive).
 
 Reserved Infix "⤳h" (at level 60, no associativity).
 Reserved Infix "⇒" (at level 60, no associativity).
 Reserved Infix "⇒n" (at level 60, no associativity).
+
+Fixpoint ne a :=
+  match a with
+  | var_tm _ => true
+  | tAbs _ => false
+  | tApp a b => ne a && nf b
+  end
+with nf a :=
+  match a with
+  | var_tm _ => true
+  | tAbs a => nf a
+  | tApp a b => ne a && nf b
+  end.
+
+Lemma ne_is_nfb a : ne a ==> nf a.
+Proof. elim : a; hauto lqb:on. Qed.
+
+Lemma ne_is_nf a : ne a -> nf a.
+Proof. sfirstorder use:ne_is_nfb b:on. Qed.
+
+Lemma ne_nf_renaming_iff a ξ : (ne a = ne (ren_tm ξ a)) /\ (nf a = nf (ren_tm ξ a)).
+Proof. elim : a ξ => //=; hauto l:on. Qed.
 
 Definition isAbs a :=
   match a with
@@ -13,10 +35,15 @@ Definition isAbs a :=
   end.
 
 Inductive ERed : tm -> tm -> Prop :=
-| ER_App a0 a1 b :
+| ER_App0 a0 a1 b :
   ~~ isAbs a0 ->
   a0 ⤳h a1 ->
   tApp a0 b ⤳h tApp a1 b
+
+| ER_App1 a b0 b1 :
+  ne a ->
+  b0 ⤳h b1 ->
+  tApp a b0 ⤳h tApp a b1
 
 | ER_AppAbs a b :
   tApp (tAbs a) b ⤳h subst_tm (b..) a
@@ -92,6 +119,9 @@ Proof.
   - hauto lq:on ctrs:Par use:morphing_suc.
 Qed.
 
+Lemma Par_refl a : a ⇒ a.
+Proof. elim : a; hauto lq:on ctrs:Par. Qed.
+
 (* Parallel, non-essential reduction *)
 Inductive NPar : tm -> tm -> Prop :=
 | PN_Var i :
@@ -106,15 +136,24 @@ Inductive NPar : tm -> tm -> Prop :=
   a0 ⇒n a1 ->
   tAbs a0 ⇒n tAbs a1
 
-| PN_App a0 a1 b0 b1 :
+| PN_App0 a0 a1 b0 b1 :
+  ~~ ne a0 ->
   a0 ⇒n a1 ->
   b0 ⇒ b1 ->
   tApp a0 b0 ⇒n tApp a1 b1
 
+| PN_App1 a b0 b1 :
+  ne a ->
+  b0 ⇒n b1 ->
+  tApp a b0 ⇒n tApp a b1
+
 where "a ⇒n b":= (NPar a b).
 
 Lemma NPar_Par a b : a ⇒n b -> a ⇒ b.
-Proof. induction 1; hauto lq:on ctrs:Par. Qed.
+Proof. induction 1; hauto lq:on ctrs:Par use:Par_refl. Qed.
+
+Lemma ERed_Par a b : a ⤳h b -> a ⇒ b.
+Proof. induction 1; hauto lq:on ctrs:Par use:Par_refl. Qed.
 
 Lemma NPar_renaming a b :
   a ⇒n b ->
@@ -125,7 +164,8 @@ Proof.
   - sfirstorder.
   - hauto lq:on ctrs:NPar use:Par_renaming.
   - hauto lq:on ctrs:NPar.
-  - hauto lq:on ctrs:NPar use:Par_renaming.
+  - hauto lq:on ctrs:NPar use:Par_renaming, ne_nf_renaming_iff.
+  - hauto lq:on ctrs:NPar use:Par_renaming, ne_nf_renaming_iff.
 Qed.
 
 Lemma isAbs_renaming a ξ : isAbs a = isAbs (ren_tm ξ a).
@@ -143,25 +183,10 @@ Proof.
   move => h.
   elim : a b /h.
   - hauto lq:on ctrs:ERed use:isAbs_renaming.
+  - hauto lq:on ctrs:ERed use:ne_nf_renaming_iff.
   - move => a b ξ /=.
     apply : ER_AppAbs'. by asimpl.
   - hauto lq:on ctrs:ERed.
-Qed.
-
-Notation "s ⤳*h t" := (rtc ERed s t) (at level 60, no associativity).
-
-Lemma hms_merge t a u  :
-  t ⇒n a ->
-  a ⤳h u ->
-  t ⇒ u.
-Proof.
-  move => h.
-  move : u.
-  elim : t a / h.
-  - hauto lq:on ctrs:Par inv:ERed.
-  - hauto q:on ctrs:Par inv:ERed.
-  - hauto lq:on ctrs:Par inv:ERed.
-  - hauto lq:on inv:NPar, ERed ctrs:Par use:NPar_Par.
 Qed.
 
 (* Takahashi's *-sequence *)
@@ -185,22 +210,120 @@ Proof.
     hauto lq:on ctrs:starseq use:NPar_renaming, Par_renaming, ERed_renaming.
 Qed.
 
-Lemma starseq_app_cong M N P Q :
-  starseq M N ->
-  P ⇒ Q ->
-  starseq (tApp M P) (tApp N Q).
+Lemma ne_par_id a b : a ⇒ b -> (ne a || nf a) -> a = b.
 Proof.
-  move => h. move : P Q. elim : M N / h.
-  - sfirstorder use:S_Refl, PN_App.
-  - move => M P N hMP hMN hPN ih R Q hRQ.
-    case E : (isAbs M).
-    + apply S_Refl.
-      case : M hMP hMN E=>//.
-      move => M.
-      elim/ered_inv=>//_ a0 b0 hab0 [?] ? h _. subst.
-      hauto lq:on inv:Par ctrs:NPar.
-    + hauto lq:on ctrs:starseq, NPar, Par, ERed.
+  move => h.
+  elim : a b /h => //=.
+  - sfirstorder lqb:on.
+  - hauto lqb:on.
 Qed.
+
+(* Lemma starseq_app_cong0 M N P Q : *)
+(*   M ⇒n N -> *)
+(*   P ⇒ Q -> *)
+(*   starseq (tApp M P) (tApp N Q). *)
+(* Proof. *)
+(*   move => h. move : P Q. elim : M N / h. *)
+(*   - move => M N hMN P Q hPQ. *)
+(*     apply S_Refl. *)
+
+(* Lemma starseq_app_cong M N P Q : *)
+(*   starseq M N -> *)
+(*   P ⇒n Q -> *)
+(*   starseq (tApp M P) (tApp N Q). *)
+(* Proof. *)
+(*   move => h. move : P Q. elim : M N / h. *)
+(*   - move => M N hMN P Q hPQ. *)
+(*     best. *)
+
+(*   - move => M P N hMP hMN hPN ih R Q hRQ. *)
+(*     case E : (isAbs M). *)
+(*     + apply S_Refl. *)
+(*       case : M hMP hMN E=>//. *)
+(*       move => M. *)
+(*       elim/ered_inv=>//_ a0 b0 hab0 [?] ? h _. subst. *)
+(*       hauto lq:on inv:Par ctrs:NPar. *)
+(*     + hauto lq:on ctrs:starseq, NPar, Par, ERed. *)
+(* Qed. *)
+
+Lemma starseq_app_cong1 a b0 b1 :
+  ne a ->
+  starseq b0 b1 ->
+  starseq (tApp a b0) (tApp a b1).
+Proof.
+  move => + h. move : a.
+  elim : b0 b1 / h.
+  - hauto lq:on ctrs:starseq, NPar.
+  - hauto lq:on use:Par_refl ctrs:ERed, Par, starseq.
+Qed.
+
+Lemma starseq_app_cong00 a0 a1 b0 b1 :
+  ~~ ne a0 ->
+  a0 ⇒n a1 ->
+  starseq b0 b1 ->
+  starseq (tApp a0 b0) (tApp a1 b1).
+Proof.
+  move => + + h. move : a0 a1. elim:b0 b1/h .
+  - hauto lq:on use:NPar_Par ctrs:starseq, NPar.
+  - hauto lq:on use:Par_refl, NPar_Par ctrs:ERed, Par, starseq, NPar.
+Qed.
+
+(* Erase the information about one step par from starseq *)
+Lemma starseq_erase a b (h : starseq a b) :
+  exists u, rtc ERed a u /\ u ⇒n b.
+Proof.
+  elim : a b /h; hauto lq:on ctrs:rtc.
+Qed.
+
+Lemma starseq_par a b (h : starseq a b) :
+  a ⇒ b.
+Proof.
+  elim : a b /h; sfirstorder use:NPar_Par.
+Qed.
+
+
+
+Lemma starseq_app_cong a0 a1 b0 b1 :
+  starseq a0 a1 ->
+  starseq b0 b1 ->
+  starseq (tApp a0 b0) (tApp a1 b1).
+Proof.
+  move => h. move : b0 b1. elim: a0 a1 /h.
+  - move => a0 a1 ha b0 b1 hb.
+    case E : (ne a0).
+    + have ? : a1 = a0 by hauto q:on use:NPar_Par, ne_par_id. subst.
+      sfirstorder use:starseq_app_cong1.
+    + hauto lq:on use:starseq_app_cong00.
+  - move => a a0 a1 ha0 ha1 ha iha b0 b1 h.
+    case E : (isAbs a) => //=.
+    + have : ~~ ne a by  move : E; clear; case : a => //=.
+      case : a E ha0 ha1 => //=.
+      hauto inv:ERed, Par use:starseq_par, S_Refl, PN_AppAbs.
+    + case E0 : (ne a).
+      * have ? : a0 = a by admit. subst.
+        apply iha=>//.
+      * apply S_Step with (P := tApp a0 b0).
+        hauto lq:on ctrs:ERed.
+        sfirstorder use: P_App, starseq_par.
+        sfirstorder.
+Admitted.
+
+Lemma hms_split t s (h : t ⇒ s) :
+  starseq t s.
+Proof.
+  elim : t s /h .
+  - hauto lq:on ctrs:NPar, starseq.
+  - eauto using starseq_app_cong.
+  - move => a0 a1 b0 b1 ha iha hb ihb.
+    apply : S_Step.
+    by apply ER_AppAbs.
+    by apply P_AppAbs.
+    hauto lq:on ctrs:starseq inv:nat use:ipar_starseq_morphing.
+  - eauto using starseq_abs_cong.
+Qed.
+
+
+
 
 Lemma starseq_abs_cong M N
   (h : starseq M N) :
@@ -254,26 +377,21 @@ Proof.
     (* renaming *)
 Qed.
 
-Lemma hms_split t s (h : t ⇒ s) :
-  starseq t s.
+Lemma hms_merge t a u  :
+  t ⇒n a ->
+  a ⤳h u ->
+  t ⇒ u.
 Proof.
-  elim : t s /h .
-  - hauto lq:on ctrs:NPar, starseq.
-  - eauto using starseq_app_cong.
-  - move => a0 a1 b0 b1 ha iha hb ihb.
-    apply : S_Step.
-    by apply ER_AppAbs.
-    by apply P_AppAbs.
-    hauto lq:on ctrs:starseq inv:nat use:ipar_starseq_morphing.
-  - eauto using starseq_abs_cong.
+  move => h.
+  move : u.
+  elim : t a / h.
+  - hauto lq:on ctrs:Par inv:ERed.
+  - hauto q:on ctrs:Par inv:ERed.
+  - hauto lq:on ctrs:Par inv:ERed.
+  - hauto lq:on inv:NPar, ERed ctrs:Par use:NPar_Par.
 Qed.
 
-(* Erase the information about one step par from starseq *)
-Lemma starseq_erase a b (h : starseq a b) :
-  exists u, a ⤳*h u /\ u ⇒n b.
-Proof.
-  elim : a b /h; hauto lq:on ctrs:rtc.
-Qed.
+
 
 Lemma local_postponement t a u  :
   t ⇒n a ->
